\documentclass{article}
\usepackage[utf8]{inputenc}
\usepackage{amsmath}
\usepackage{amsfonts}
\usepackage{graphicx}
\graphicspath{ {./images/} }

\title{Difference equations}
\author{Gabriel Aguiar}
\date{October 2019}

\begin{document}

\maketitle

Difference equations represent the discrete description of ordinary differential equations. Let's look at some formulations to study them:

\begin{itemize}

\item Operator $\Delta$ definition:

$\Delta y(x) \equiv \Delta_{h} y(x) \equiv y(x + h) - y(x)$

$\Delta^{2} y(x) \equiv \Delta_{h}^{2} y(x) \equiv \Delta_{h} [\Delta_{h} y(x)] = y(x + 2h) - 2y(x + h) + y(x)$

\item Difference equation definition:

$F(x,\Delta y(x),\Delta^{2} y(x),...,\Delta^{n}y(x)) = 0$

\item Theorem:

$\Delta \sum\limits_{l = 1}^{k} \; c_{l} \; y^{l} (x) = \sum\limits_{l = 1}^{k} \; c_{l} \; \Delta y^{l} (x)$

That way, $\Delta$ is a linear operator.

\item Theorem:

$y(x) = \sum\limits_{l = 0}^{n} \; a_{l} \; x^{l} \Rightarrow \Delta^{n} y(x) = n! \; h^{n} \; a_{n}$

$\Delta^{n + 1} y(x) = 0$

\item Operator $E$ definition:

$Ey(x) \equiv y(x + h)$

\item Operator $I$ definition:

$Iy(x) \equiv y(x)$

\item Observations:

$\Delta y(x) = Ey(x) - Iy(x)$, $\forall y$

$\Delta \equiv E - I$

$E^{2} y = E[Ey(x)] = E[y(x + h)] = y(x + 2h)$

$E^{k} y = y(x + kh)$

\item Factorial function definition

$x^{(n)} \equiv x(x - h)(x - 2h) ... [x - (n - 1)h]$

$x^{(0)} \equiv 1$

$\Delta x^{(n)} = (x + h)^{(n)} - x^{(n)} = nhx^{(n-1)}$

\item Theorem:

$\Delta [u(x)v(x)] = Eu(x) \; \Delta v(x) + Ev(x) \; \Delta u(x)$

\item Theorem:

$\Delta^{n} y(x) = \sum\limits_{k = 0}^{n} \; \binom{n}{k} (-1)^{n - k} \; E^{k} y(x)$, $\forall y$

\item Observations:

$\Delta^{n} y(x) = \sum\limits_{k = 0}^{n} \; \binom{n}{k} (-1)^{n - k} \; y(x + kh)$

$\Delta^{n} \equiv \sum\limits_{k = 0}^{n} \; \binom{n}{k} (-1)^{n - k} \; E^{k}$

\item Theorem:

$E^{n} \equiv (\Delta + I)^{n} \equiv \sum\limits_{k = 0}^{n} \; \binom{n}{k} \Delta^{k}$

\item Undefined sum:

If $Y$ is the function such that $\Delta Y(x) = y(x)$, then $\Delta^{-1} y(x) = Y(x)$.

\item Observations:

$\Delta x^{(n)} = nhx^{(n - 1)} \Rightarrow \Delta^{-1} x^{(n - 1)} = \frac{1}{nh} \; x^{(n)} + \Pi$

$\Delta [\Delta^{n - 1} y(x)] = \Delta^{n} y(x)$

\item Theorem:

$\Delta (\frac{u(x)}{v(x)}) = \frac{1}{v(x) Ev(x)} \; v(x) \Delta u(x) - u(x) \Delta v(x)$
    
\end{itemize}

\end{document}